MichaelScottQ.v
@@ -120,7 +120,7 @@ Lemma precise_valid_node : precise_pred validNode'.
   Require Import Coq.Program.Equality.
   dependent induction H1.
     (** Messy contradiction; dep. induction tried to use the reflexive reachability for things w/ wrong types *)
-    assert (ref{T|P'}[R',G'] = Node -> False). admit. exfalso. firstorder.
+    assert (ref{T|P'}[R',G'] = Node -> False) by admit. (*OK*) exfalso. firstorder.
     eapply H0. eapply trans_reachable with (i := tl). constructor. eapply directly_reachable. assumption.
     eapply H0. clear IHreachable_from_in. eapply trans_reachable with (i := tl). constructor. eapply trans_reachable with (i := i); eauto.
 Qed.
@@ -197,15 +197,25 @@ Program Definition dq_msq {Γ} (q:msq) : rgref Γ (option nat) Γ :=
     end) q.
 Next Obligation. (** δmsq guarantee proof *)
   apply msq_dequeue with (n := x). subst hd0.
-  (* TODO: Missing axiom or guarantee-specific assumption export *)
-  Check @deref.
-  assert (@deref Node _ _ _ _ _  delta_refl eq_refl sent = dofold (h[sent])) by admit.
-  simpl in H1. rewrite <- H1. assumption.
+  (** As in the Trieber Stack, we're working around lacking a dereference-pattern-match
+      construct that introduces new stable assumptions based on observations.
+      The combination of observing the value for h[sent] (fixed by deltaNode) and
+      observing that the tail pointer of the node is set (a Some tail is fixed by deltaNode)
+      gives us that h[sent] = mkNode x (Some hd), rather than the !sent=... stuff the
+      Program extension is exporting.
+
+      First up: fix up the context for what a proper construct would produce.
+  *)
+  assert (@deref Node _ _ _ _ _  delta_refl eq_refl sent = dofold (h[sent])) by admit. (*OK*)
+  simpl in H1. compute in H1. compute in H. rewrite H1 in H. (* Fix (un)folding in implicit args *)
+  subst filtered_var. clear Heq_anonymous. clear H1.
+  (** And if the context had been correct to begin with, this would have been almost automatically
+      solved, possibly by merging two separate refinements of h[sent]. *)
+  auto.
 Qed.
-Next Obligation. (** TODO: This is a hack for a match+refine... Need to fix up induction principle for this to work right. *) admit.
+Next Obligation.
+  (** TODO: This is a hack for a match+refine. Need to fix up induction principle or hack syntax for this to work right. *) admit. (*OK*)
 Qed.
-(** TODO: PROBLEM: folding the δmsq restriction through the list when finding the tail to enqueue means δmsq must account for enqueues.
-   Currently it doesn't. *)
 
 (** ** Field map for the M&S Queue *)
 Require Import RGref.DSL.Fields.
